src/program_proof/pav/client.v
@@ -131,7 +131,7 @@ Lemma wp_checkMemb ptr_vrf_pk vrf_pk (uid ver : w64) sl_dig (dig : list w8) ptr_
     "Hown_memb" ∷ Memb.own ptr_memb memb ∗
     "Herr" ∷ (if err then True else
       "#His_label" ∷ is_map_label vrf_pk uid ver label ∗
-      "#His_commit" ∷ is_commit memb.(Memb.PkOpen).(CommitOpen.Pk) comm ∗
+      "#His_commit" ∷ is_commit memb.(Memb.PkOpen).(CommitOpen.Val) comm ∗
       "#Hhas_merk_proof" ∷ is_merkle_entry label
         (Some (MapValPre.encodesF $ MapValPre.mk memb.(Memb.EpochAdded) comm)) dig)
   }}}.
@@ -212,7 +212,7 @@ Lemma wp_Client__Put ptr_c c sl_pk d0 (pk : list w8) :
     "Herr" ∷ if err.(ClientErr.Err) then
       "Hown_cli" ∷ Client.own ptr_c c
     else
-      let new_c := set Client.next_ver (word.add (W64 1))
+      let new_c := set Client.next_ver (λ x, (word.add x (W64 1)))
         (set Client.next_epoch (λ _, (word.add ep (W64 1))) c) in
       "Hown_cli" ∷ Client.own ptr_c new_c ∗
       "#His_put_post" ∷ is_put_post c.(Client.γ) c.(Client.serv_vrf_pk)
@@ -221,7 +221,79 @@ Lemma wp_Client__Put ptr_c c sl_pk d0 (pk : list w8) :
       "%Hnoof_eq" ∷ ⌜ uint.Z (word.add ep (W64 1)) = (uint.Z ep + 1)%Z ⌝ ∗
       "%Hgt_ep" ∷ ⌜ uint.Z c.(Client.next_epoch) ≤ uint.Z ep ⌝
   }}}.
-Proof. Admitted.
+Proof.
+  iIntros (Φ) "H HΦ". iNamed "H". iNamed "Hown_cli". rewrite /Client__Put.
+  wp_apply wp_allocStruct; [val_ty|]. iIntros (?) "H".
+  iAssert (ClientErr.own _ (ClientErr.mk None _) c.(Client.serv_sig_pk)) with "[H]" as "Hown_std_err".
+  { iDestruct (struct_fields_split with "H") as "H". iNamed "H". iFrame. }
+  do 2 wp_loadField.
+  wp_apply (wp_CallServPut with "[$Hown_servCli $Hsl_pk]").
+  iIntros (?????? err0). iNamed 1. destruct err0.
+  { wp_pures. iApply "HΦ". by iFrame "∗∗#%". }
+  iNamed "Herr". iPoseProof "Hown_dig" as "H". iNamed "H".
+  (* TODO: wp_pures takes a long time for some reason. *)
+  wp_pures. do 2 wp_loadField.
+  wp_apply (wp_checkDig with "[$Hsl_servSigPk $Hown_sd $Hown_sd_refs $His_sd $Hown_dig]").
+  iIntros (? err1). iNamed 1. iNamedSuffix "Hown_err" "1". wp_loadField.
+  destruct (err1.(ClientErr.Err)).
+  { wp_pures. iApply ("HΦ" $! _ _ (ClientErr.mk _ true)).
+    iClear "Hown_std_err". by iFrame "∗#%". }
+  iClear "Hptr_evid1 Hptr_err1 Hevid1". iNamed "Herr".
+  do 2 wp_loadField. wp_if_destruct.
+  { wp_pures. iApply "HΦ". by iFrame "∗∗#%". }
+  rename Heqb into Hfresh_ep. do 4 wp_loadField.
+  wp_apply (wp_checkMemb with "[$Hown_vrf_pk $Hsl_Dig $Hown_memb]").
+  iIntros (???). iNamed 1. wp_if_destruct.
+  { wp_pures. iApply "HΦ". by iFrame "∗∗#%". }
+  iNamedSuffix "Herr" "_memb". iNamed "Hown_memb".
+  do 2 wp_loadField. wp_if_destruct.
+  { wp_pures. iApply "HΦ". by iFrame "∗∗#%". }
+  rewrite -Heqb0 {Heqb0}. iNamedSuffix "Hown_pk_open" "_open0". do 2 wp_loadField.
+  wp_apply (wp_BytesEqual sl_pk sl_val with "[$Hsl_pk $Hsl_val_open0]").
+  iIntros "[Hsl_pk _]". wp_if_destruct.
+  { wp_pures. iApply "HΦ". by iFrame "∗∗#%". }
+  rewrite -Heqb {Heqb}. do 4 wp_loadField.
+  wp_apply (wp_checkNonMemb with "[$Hown_vrf_pk $Hsl_Dig $Hown_nonmemb]").
+  iIntros (??). iNamed 1. wp_if_destruct.
+  { wp_pures. iApply "HΦ". by iFrame "∗∗#%". }
+  iNamedSuffix "Herr" "_nonmemb". do 2 wp_loadField.
+  wp_apply (wp_MapInsert_to_val with "[$Hown_sd_refs]").
+  iIntros "Hown_sd_refs". wp_loadField. wp_storeField. wp_loadField.
+  wp_apply wp_SumAssumeNoOverflow. iIntros "%Hnoof_ver".
+  wp_storeField. wp_loadField.
+  wp_apply wp_allocStruct; [val_ty|]. iIntros (?) "H".
+  iDestruct (struct_fields_split with "H") as "H". iNamed "H".
+  wp_pures. iApply ("HΦ" $! _ _ (ClientErr.mk None false)).
+  iDestruct (big_sepM2_insert_2 (λ _ x y, SigDig.own x y) _ _ dig.(SigDig.Epoch)
+    with "Hown_dig Hown_sd") as "Hnew_own_sd".
+  iDestruct (big_sepM_insert_2 (λ _ x, is_SigDig x _) _ dig.(SigDig.Epoch)
+    with "His_dig His_sd") as "Hnew_is_sd".
+  iClear "Hown_sd His_sd Hown_dig His_dig".
+
+  (* grow ghost digs. *)
+  set (digs ++ (replicate (uint.nat dig.(SigDig.Epoch) - length digs) None) ++
+    [Some dig.(SigDig.Dig)]) as new_digs.
+  iMod (mono_list_auth_own_update new_digs with "Hown_digs") as "[Hown_digs #Hlb]".
+  { by apply prefix_app_r. }
+  iDestruct (mono_list_idx_own_get (uint.nat dig.(SigDig.Epoch)) with "Hlb") as "#Hlook_gdigs".
+  { rewrite lookup_app_r; [|word].
+    rewrite lookup_app_r; rewrite length_replicate; [|done].
+    apply list_lookup_singleton_Some. split; [lia|done]. }
+  iFrame "∗#". iIntros "!> !% //".
+  repeat try split; [idtac|idtac|idtac|word..].
+  - intros ep ? Hlook_digs.
+    apply lookup_app_Some in Hlook_digs as [Hlook_digs|[? Hlook_digs]].
+    { rewrite lookup_insert_ne. 2: { apply lookup_lt_Some in Hlook_digs. word. }
+      opose proof (Hagree_digs_sd _ _ Hlook_digs) as [? Hlook_sd]. naive_solver. }
+    apply lookup_app_Some in Hlook_digs as [Hlook_digs|[Heq0 Hlook_digs]].
+    { apply lookup_replicate in Hlook_digs. naive_solver. }
+    apply list_lookup_singleton_Some in Hlook_digs as [Heq1 Hlook_digs].
+    rewrite length_replicate in Heq0 Heq1.
+    assert (ep = dig.(SigDig.Epoch)) as -> by word.
+    rewrite lookup_insert. destruct dig. naive_solver.
+  - subst new_digs. rewrite app_assoc last_snoc. naive_solver.
+  - rewrite !length_app length_replicate. simpl. word.
+Qed.
 
 Definition is_selfmon_post cli_γ serv_vrf_pk uid ver (ep : w64) : iProp Σ :=
   "#His_bound" ∷ is_cli_entry cli_γ serv_vrf_pk ep uid ver None.
@@ -342,7 +414,8 @@ Qed.
 Definition is_get_post cli_γ serv_vrf_pk uid (ep : w64) (lat : lat_val_ty) : iProp Σ :=
   ∃ (vals : list opaque_map_val_ty),
   "#Hlat_pk_commit" ∷ lat_pk_commit lat (last vals) ∗
-  "#Hhist" ∷ ([∗ list] ver ↦ val ∈ vals, is_cli_entry cli_γ serv_vrf_pk ep uid ver (Some val)) ∗
+  "#Hhist" ∷ ([∗ list] ver ↦ val ∈ vals,
+    is_cli_entry cli_γ serv_vrf_pk ep uid ver (Some val)) ∗
   "#His_bound" ∷ is_cli_entry cli_γ serv_vrf_pk ep uid (W64 $ length vals) None.
 
 Lemma wp_Client__Get ptr_c c uid :
